High level Merkle tree hash function parameterization, part 2

secure_api/merkle_tree/MerkleTree.New.High.Correct.Base.fst
@@ -6,8 +6,8 @@ open FStar.Seq
 
 module S = FStar.Seq
 
-module MTH = MerkleTree.New.High
 module MTS = MerkleTree.Spec
+open MerkleTree.New.High
 
 #set-options "--z3rlimit 40 --max_fuel 0 --max_ifuel 0"
 
@@ -36,7 +36,7 @@ let seq_tail_cons #a x s = ()
 
 // Invariants of internal hashes
 
-val empty_hashes: (#hsz:pos) -> (len:nat) -> GTot (hs:MTH.hashess #hsz {S.length hs = len})
+val empty_hashes: (#hsz:pos) -> (len:nat) -> GTot (hs:hashess #hsz {S.length hs = len})
 let empty_hashes #hsz len = S.create len S.empty
 
 val empty_hashes_head:
@@ -58,7 +58,7 @@ val mt_hashes_lth_inv:
   #hsz:pos ->
   lv:nat{lv <= 32} ->
   j:nat{j < pow2 (32 - lv)} ->
-  fhs:MTH.hashess #hsz {S.length fhs = 32} ->
+  fhs:hashess #hsz {S.length fhs = 32} ->
   GTot Type0 (decreases (32 - lv))
 let rec mt_hashes_lth_inv #hsz lv j fhs =
   if lv = 32 then true
@@ -78,8 +78,8 @@ let rec mt_hashes_lth_inv_empty #hsz lv =
 val mt_hashes_next_rel:
   #hsz:pos -> #f:MTS.tag_fun_t #hsz ->
   j:nat ->
-  hs:MTH.hashes #hsz {S.length hs = j} ->
-  nhs:MTH.hashes #hsz {S.length nhs = j / 2} ->
+  hs:hashes #hsz {S.length hs = j} ->
+  nhs:hashes #hsz {S.length nhs = j / 2} ->
   GTot Type0
 let mt_hashes_next_rel #hsz #f j hs nhs =
   forall (i:nat{i < j / 2}).
@@ -93,7 +93,7 @@ val mt_hashes_inv:
   #hsz:pos -> #f:MTS.tag_fun_t #hsz ->
   lv:nat{lv < 32} ->
   j:nat{j < pow2 (32 - lv)} ->
-  fhs:MTH.hashess #hsz {S.length fhs = 32 /\ mt_hashes_lth_inv lv j fhs} ->
+  fhs:hashess #hsz {S.length fhs = 32 /\ mt_hashes_lth_inv lv j fhs} ->
   GTot Type0 (decreases (32 - lv))
 let rec mt_hashes_inv #hsz #f lv j fhs =
   if lv = 31 then true
@@ -116,8 +116,8 @@ val mt_hashes_lth_inv_equiv:
   #hsz:pos -> #f:MTS.tag_fun_t #hsz ->
   lv:nat{lv < 32} ->
   j:nat{j < pow2 (32 - lv)} ->
-  fhs1:MTH.hashess{S.length fhs1 = 32} ->
-  fhs2:MTH.hashess{S.length fhs2 = 32} ->
+  fhs1:hashess{S.length fhs1 = 32} ->
+  fhs2:hashess{S.length fhs2 = 32} ->
   Lemma (requires mt_hashes_lth_inv lv j fhs1 /\
                   S.equal (S.slice fhs1 lv 32) (S.slice fhs2 lv 32))
         (ensures mt_hashes_lth_inv #hsz lv j fhs2)
@@ -133,8 +133,8 @@ val mt_hashes_inv_equiv:
   #hsz:pos -> #f:MTS.tag_fun_t #hsz ->
   lv:nat{lv < 32} ->
   j:nat{j < pow2 (32 - lv)} ->
-  fhs1:MTH.hashess #hsz {S.length fhs1 = 32 /\ mt_hashes_lth_inv lv j fhs1} ->
-  fhs2:MTH.hashess #hsz {S.length fhs2 = 32 /\ mt_hashes_lth_inv lv j fhs2} ->
+  fhs1:hashess #hsz {S.length fhs1 = 32 /\ mt_hashes_lth_inv lv j fhs1} ->
+  fhs2:hashess #hsz {S.length fhs2 = 32 /\ mt_hashes_lth_inv lv j fhs2} ->
   Lemma (requires mt_hashes_inv #_ #f lv j fhs1 /\
                   S.equal (S.slice fhs1 lv 32) (S.slice fhs2 lv 32))
         (ensures mt_hashes_inv #_ #f lv j fhs2)
@@ -147,9 +147,9 @@ let rec mt_hashes_inv_equiv #hsz #f lv j fhs1 fhs2 =
 
 val merge_hs:
   #hsz:pos -> #f:MTS.tag_fun_t #hsz ->
-  hs1:MTH.hashess #hsz ->
-  hs2:MTH.hashess #hsz {S.length hs1 = S.length hs2} ->
-  GTot (mhs:MTH.hashess #hsz {S.length mhs = S.length hs1})
+  hs1:hashess #hsz ->
+  hs2:hashess #hsz {S.length hs1 = S.length hs2} ->
+  GTot (mhs:hashess #hsz {S.length mhs = S.length hs1})
        (decreases (S.length hs1))
 let rec merge_hs #hsz #f hs1 hs2 =
   if S.length hs1 = 0 then S.empty
@@ -165,8 +165,8 @@ let rec merge_hs_empty #hsz #f len =
   if len = 0 then ()
   else (empty_hashes_head #hsz len;
        empty_hashes_tail #hsz len;
-       assert (S.equal (S.append #(MTH.hash #hsz) S.empty S.empty)
-                       (S.empty #(MTH.hash #hsz)));
+       assert (S.equal (S.append #(hash #hsz) S.empty S.empty)
+                       (S.empty #(hash #hsz)));
        assert (S.equal (merge_hs #_ #f (empty_hashes len) (empty_hashes len))
                        (S.cons S.empty
                                (merge_hs #_ #f (empty_hashes (len - 1))
@@ -175,8 +175,8 @@ let rec merge_hs_empty #hsz #f len =
 
 val merge_hs_index:
   #hsz:pos -> #f:MTS.tag_fun_t #hsz ->
-  hs1:MTH.hashess ->
-  hs2:MTH.hashess{S.length hs1 = S.length hs2} ->
+  hs1:hashess ->
+  hs2:hashess{S.length hs1 = S.length hs2} ->
   i:nat{i < S.length hs1} ->
   Lemma (requires True)
         (ensures S.equal (S.index (merge_hs #_ #f hs1 hs2) i)
@@ -190,10 +190,10 @@ let rec merge_hs_index #hsz #f hs1 hs2 i =
 
 val merge_hs_slice_equal:
   #hsz:pos -> #f:MTS.tag_fun_t #hsz ->
-  ahs1:MTH.hashess #hsz ->
-  ahs2:MTH.hashess #hsz {S.length ahs1 = S.length ahs2} ->
-  bhs1:MTH.hashess #hsz ->
-  bhs2:MTH.hashess #hsz {S.length bhs1 = S.length bhs2} ->
+  ahs1:hashess #hsz ->
+  ahs2:hashess #hsz {S.length ahs1 = S.length ahs2} ->
+  bhs1:hashess #hsz ->
+  bhs2:hashess #hsz {S.length bhs1 = S.length bhs2} ->
   i:nat -> j:nat{i <= j && j <= S.length ahs1 && j <= S.length bhs1} ->
   Lemma (requires S.equal (S.slice ahs1 i j) (S.slice bhs1 i j) /\
                   S.equal (S.slice ahs2 i j) (S.slice bhs2 i j))
@@ -208,10 +208,10 @@ let rec merge_hs_slice_equal #_ #f ahs1 ahs2 bhs1 bhs2 i j =
 
 val merge_hs_upd:
   #hsz:pos -> #f:MTS.tag_fun_t #hsz ->
-  hs1:MTH.hashess #hsz ->
-  hs2:MTH.hashess #hsz {S.length hs1 = S.length hs2} ->
+  hs1:hashess #hsz ->
+  hs2:hashess #hsz {S.length hs1 = S.length hs2} ->
   i:nat{i < S.length hs1} ->
-  v1:MTH.hashes #hsz -> v2:MTH.hashes #hsz ->
+  v1:hashes #hsz -> v2:hashes #hsz ->
   Lemma (requires S.equal (S.append (S.index hs1 i) (S.index hs2 i))
                           (S.append v1 v2))
         (ensures S.equal (merge_hs #_ #f hs1 hs2)
@@ -226,11 +226,11 @@ val mt_olds_inv:
   #hsz:pos -> #f:MTS.tag_fun_t #hsz ->
   lv:nat{lv <= 32} ->
   i:nat ->
-  olds:MTH.hashess #hsz {S.length olds = 32} ->
+  olds:hashess #hsz {S.length olds = 32} ->
   GTot Type0 (decreases (32 - lv))
 let rec mt_olds_inv #_ #f lv i olds =
   if lv = 32 then true
-  else (let ofs = MTH.offset_of i in
+  else (let ofs = offset_of i in
        S.length (S.index olds lv) == ofs /\
        mt_olds_inv #_ #f (lv + 1) (i / 2) olds)
 
@@ -238,8 +238,8 @@ val mt_olds_inv_equiv:
   #hsz:pos -> #f:MTS.tag_fun_t #hsz ->
   lv:nat{lv <= 32} ->
   i:nat ->
-  olds1:MTH.hashess #hsz {S.length olds1 = 32} ->
-  olds2:MTH.hashess #hsz {S.length olds2 = 32} ->
+  olds1:hashess #hsz {S.length olds1 = 32} ->
+  olds2:hashess #hsz {S.length olds2 = 32} ->
   Lemma (requires mt_olds_inv #_ #f lv i olds1 /\
                   S.equal (S.slice olds1 lv 32) (S.slice olds2 lv 32))
         (ensures mt_olds_inv #_ #f lv i olds2)
@@ -254,8 +254,8 @@ val mt_olds_hs_lth_inv_ok:
   lv:nat{lv <= 32} ->
   i:nat ->
   j:nat{i <= j /\ j < pow2 (32 - lv)} ->
-  olds:MTH.hashess #hsz {S.length olds = 32 /\ mt_olds_inv #_ #f lv i olds} ->
-  hs:MTH.hashess #hsz {S.length hs = 32 /\ MTH.hs_wf_elts #hsz lv hs i j} ->
+  olds:hashess #hsz {S.length olds = 32 /\ mt_olds_inv #_ #f lv i olds} ->
+  hs:hashess #hsz {S.length hs = 32 /\ hs_wf_elts #hsz lv hs i j} ->
   Lemma (requires True)
         (ensures mt_hashes_lth_inv #hsz lv j (merge_hs #_ #f olds hs))
         (decreases (32 - lv))
@@ -268,8 +268,8 @@ val mt_olds_hs_inv:
   lv:nat{lv < 32} ->
   i:nat ->
   j:nat{i <= j /\ j < pow2 (32 - lv)} ->
-  olds:MTH.hashess #hsz {S.length olds = 32 /\ mt_olds_inv #_ #f lv i olds} ->
-  hs:MTH.hashess #hsz {S.length hs = 32 /\ MTH.hs_wf_elts #hsz lv hs i j} ->
+  olds:hashess #hsz {S.length olds = 32 /\ mt_olds_inv #_ #f lv i olds} ->
+  hs:hashess #hsz {S.length hs = 32 /\ hs_wf_elts #hsz lv hs i j} ->
   GTot Type0
 let mt_olds_hs_inv #hsz #f lv i j olds hs =
   mt_olds_hs_lth_inv_ok #_ #f lv i j olds hs;
@@ -319,7 +319,7 @@ let rec log2c_bound n c =
 val mt_hashes_lth_inv_log:
   #hsz:pos -> #f:MTS.tag_fun_t #hsz ->
   j:nat ->
-  fhs:MTH.hashess #hsz {S.length fhs = log2c j} ->
+  fhs:hashess #hsz {S.length fhs = log2c j} ->
   GTot Type0 (decreases j)
 let rec mt_hashes_lth_inv_log #_ #f j fhs =
   if j = 0 then true
@@ -331,7 +331,7 @@ let rec mt_hashes_lth_inv_log #_ #f j fhs =
 val mt_hashes_lth_inv_log_next:
   #hsz:pos -> #f:MTS.tag_fun_t #hsz ->
   j:nat{j > 1} ->
-  fhs:MTH.hashess #hsz {S.length fhs = log2c j} ->
+  fhs:hashess #hsz {S.length fhs = log2c j} ->
   Lemma (requires mt_hashes_lth_inv_log #_ #f j fhs)
         (ensures S.length (S.head fhs) == j /\
                  S.length (S.head (S.tail fhs)) == j / 2)
@@ -340,7 +340,7 @@ let mt_hashes_lth_inv_log_next #_ #_ _ _ = ()
 val mt_hashes_inv_log:
   #hsz:pos -> #f:MTS.tag_fun_t #hsz ->
   j:nat ->
-  fhs:MTH.hashess #hsz {S.length fhs = log2c j /\ mt_hashes_lth_inv_log #_ #f j fhs} ->
+  fhs:hashess #hsz {S.length fhs = log2c j /\ mt_hashes_lth_inv_log #_ #f j fhs} ->
   GTot Type0 (decreases j)
 let rec mt_hashes_inv_log #hsz #f j fhs =
   if j <= 1 then true
@@ -351,7 +351,7 @@ val mt_hashes_lth_inv_log_converted_:
   #hsz:pos -> #f:MTS.tag_fun_t #hsz ->
   lv:nat{lv <= 32} ->
   j:nat{j < pow2 (32 - lv)} ->
-  fhs:MTH.hashess #hsz {S.length fhs = 32} ->
+  fhs:hashess #hsz {S.length fhs = 32} ->
   Lemma (requires mt_hashes_lth_inv #hsz lv j fhs)
         (ensures (log2c_bound j (32 - lv);
                   mt_hashes_lth_inv_log #_ #f j (S.slice fhs lv (lv + log2c j))))
@@ -364,7 +364,7 @@ let rec mt_hashes_lth_inv_log_converted_ #_ #f lv j fhs =
 val mt_hashes_lth_inv_log_converted:
   #hsz:pos -> #f:MTS.tag_fun_t #hsz ->
   j:nat{j < pow2 32} ->
-  fhs:MTH.hashess #hsz {S.length fhs = 32} ->
+  fhs:hashess #hsz {S.length fhs = 32} ->
   Lemma (requires mt_hashes_lth_inv #hsz 0 j fhs)
         (ensures (log2c_bound j 32;
                   mt_hashes_lth_inv_log #_ #f j (S.slice fhs 0 (log2c j))))
@@ -375,7 +375,7 @@ val mt_hashes_inv_log_converted_:
   #hsz:pos -> #f:MTS.tag_fun_t #hsz ->
   lv:nat{lv <= 32} ->
   j:nat{j > 0 && j < pow2 (32 - lv)} ->
-  fhs:MTH.hashess #hsz {S.length fhs = 32 /\ mt_hashes_lth_inv #hsz lv j fhs} ->
+  fhs:hashess #hsz {S.length fhs = 32 /\ mt_hashes_lth_inv #hsz lv j fhs} ->
   Lemma (requires mt_hashes_inv #_ #f lv j fhs)
         (ensures (log2c_bound j (32 - lv);
                   mt_hashes_lth_inv_log_converted_ #_ #f lv j fhs;
@@ -391,7 +391,7 @@ let rec mt_hashes_inv_log_converted_ #_ #f lv j fhs =
 val mt_hashes_inv_log_converted:
   #hsz:pos -> #f:MTS.tag_fun_t #hsz ->
   j:nat{j > 0 && j < pow2 32} ->
-  fhs:MTH.hashess #hsz {S.length fhs = 32 /\ mt_hashes_lth_inv #hsz 0 j fhs} ->
+  fhs:hashess #hsz {S.length fhs = 32 /\ mt_hashes_lth_inv #hsz 0 j fhs} ->
   Lemma (requires mt_hashes_inv #_ #f 0 j fhs)
         (ensures (log2c_bound j 32;
                   mt_hashes_lth_inv_log_converted_ #_ #f 0 j fhs;
@@ -401,7 +401,7 @@ let mt_hashes_inv_log_converted #_ #f j fhs =
 
 val hash_seq_lift: 
   #hsz:pos -> #f:MTS.tag_fun_t #hsz ->
-  hs:MTH.hashes #hsz -> 
+  hs:hashes #hsz -> 
   GTot (shs:MTS.tags #hsz {S.length shs = S.length hs})
        (decreases (S.length hs))
 let rec hash_seq_lift #_ #f hs =
@@ -410,7 +410,7 @@ let rec hash_seq_lift #_ #f hs =
 
 val hash_seq_lift_index:
   #hsz:pos -> #f:MTS.tag_fun_t #hsz ->
-  hs:MTH.hashes #hsz ->
+  hs:hashes #hsz ->
   Lemma (requires True)
         (ensures  forall (i:nat{i < S.length hs}).
                     S.index (hash_seq_lift #_ #f hs) i == MTS.HRaw (S.index hs i))
@@ -426,7 +426,7 @@ let create_pads #hsz len = S.create len (MTS.HPad #hsz)
 
 val hash_seq_spec:
   #hsz:pos -> #f:MTS.tag_fun_t #hsz ->
-  hs:MTH.hashes #hsz {S.length hs > 0} ->
+  hs:hashes #hsz {S.length hs > 0} ->
   GTot (smt:MTS.merkle_tree #hsz (log2c (S.length hs)))
 let hash_seq_spec #_ #f hs =
   S.append (hash_seq_lift #_ #f hs)
@@ -434,7 +434,7 @@ let hash_seq_spec #_ #f hs =
 
 val hash_seq_spec_index_raw:
   #hsz:pos -> #f:MTS.tag_fun_t #hsz ->
-  hs:MTH.hashes #hsz {S.length hs > 0} ->
+  hs:hashes #hsz {S.length hs > 0} ->
   i:nat{i < S.length hs} ->
   Lemma (S.index (hash_seq_spec #_ #f hs) i == MTS.HRaw #hsz (S.index hs i))
 let hash_seq_spec_index_raw #_ #f hs i =
@@ -445,8 +445,8 @@ let hash_seq_spec_index_raw #_ #f hs i =
 val mt_hashes_next_rel_lift_even:
   #hsz:pos -> #f:MTS.tag_fun_t #hsz ->
   j:nat{j > 1} ->
-  hs:MTH.hashes #hsz {S.length hs = j} ->
-  nhs:MTH.hashes #hsz {S.length nhs = j / 2} ->
+  hs:hashes #hsz {S.length hs = j} ->
+  nhs:hashes #hsz {S.length nhs = j / 2} ->
   Lemma (requires j % 2 = 0 /\ mt_hashes_next_rel #_ #f j hs nhs)
         (ensures MTS.mt_next_rel #_ #f (log2c j)
                    (hash_seq_spec #_ #f hs) (hash_seq_spec #_ #f nhs))
@@ -457,8 +457,8 @@ let mt_hashes_next_rel_lift_even #_ #f j hs nhs =
 val mt_hashes_next_rel_lift_odd:
   #hsz:pos -> #f:MTS.tag_fun_t #hsz ->
   j:nat{j > 1} ->
-  hs:MTH.hashes #hsz {S.length hs = j} ->
-  nhs:MTH.hashes #hsz {S.length nhs = j / 2} ->
+  hs:hashes #hsz {S.length hs = j} ->
+  nhs:hashes #hsz {S.length nhs = j / 2} ->
   Lemma (requires j % 2 = 1 /\ mt_hashes_next_rel #_ #f j hs nhs)
         (ensures  MTS.mt_next_rel #_ #f (log2c j)
                    (hash_seq_spec #_ #f hs)
@@ -472,8 +472,8 @@ let mt_hashes_next_rel_lift_odd #_ #f j hs nhs =
 val mt_hashes_next_rel_next_even:
   #hsz:pos -> #f:MTS.tag_fun_t #hsz ->
   j:nat{j > 1} ->
-  hs:MTH.hashes #hsz {S.length hs = j} ->
-  nhs:MTH.hashes #hsz {S.length nhs = j / 2} ->
+  hs:hashes #hsz {S.length hs = j} ->
+  nhs:hashes #hsz {S.length nhs = j / 2} ->
   Lemma (requires j % 2 = 0 /\ mt_hashes_next_rel #_ #f j hs nhs)
         (ensures  S.equal (hash_seq_spec #_ #f nhs)
                           (MTS.mt_next_lv #_ #f #(log2c j) (hash_seq_spec #_ #f hs)))
@@ -485,8 +485,8 @@ let mt_hashes_next_rel_next_even #_ #f j hs nhs =
 
 val hash_seq_spec_full:
   #hsz:pos -> #f:MTS.tag_fun_t #hsz ->
-  hs:MTH.hashes #hsz {S.length hs > 0} ->
-  acc:MTH.hash #hsz -> actd:bool ->
+  hs:hashes #hsz {S.length hs > 0} ->
+  acc:hash #hsz -> actd:bool ->
   GTot (smt:MTS.merkle_tree #hsz (log2c (S.length hs)))
 let hash_seq_spec_full #_ #f hs acc actd =
   if actd
@@ -495,8 +495,8 @@ let hash_seq_spec_full #_ #f hs acc actd =
 
 val hash_seq_spec_full_index_raw:
   #hsz:pos -> #f:MTS.tag_fun_t #hsz ->
-  hs:MTH.hashes #hsz {S.length hs > 0} ->
-  acc:MTH.hash #hsz -> actd:bool -> i:nat{i < S.length hs} ->
+  hs:hashes #hsz {S.length hs > 0} ->
+  acc:hash #hsz -> actd:bool -> i:nat{i < S.length hs} ->
   Lemma (S.index (hash_seq_spec_full #_ #f hs acc actd) i ==
         MTS.HRaw (S.index hs i))
 let hash_seq_spec_full_index_raw #_ #f hs acc actd i =
@@ -504,16 +504,16 @@ let hash_seq_spec_full_index_raw #_ #f hs acc actd i =
 
 val hash_seq_spec_full_case_true:
   #hsz:pos -> #f:MTS.tag_fun_t #hsz ->
-  hs:MTH.hashes #hsz {S.length hs > 0} -> acc:MTH.hash #hsz ->
+  hs:hashes #hsz {S.length hs > 0} -> acc:hash #hsz ->
   Lemma (S.index (hash_seq_spec_full #_ #f hs acc true) (S.length hs) == MTS.HRaw acc)
 let hash_seq_spec_full_case_true #_ #_ _ _ = ()  
 
 val hash_seq_spec_full_even_next:
   #hsz:pos -> #f:MTS.tag_fun_t #hsz ->
   j:nat{j > 0} ->
-  hs:MTH.hashes #hsz {S.length hs = j} ->
-  nhs:MTH.hashes #hsz {S.length nhs = j / 2} ->
-  acc:MTH.hash #hsz -> actd:bool ->
+  hs:hashes #hsz {S.length hs = j} ->
+  nhs:hashes #hsz {S.length nhs = j / 2} ->
+  acc:hash #hsz -> actd:bool ->
   Lemma
     (requires j % 2 = 0 /\ mt_hashes_next_rel #_ #f j hs nhs)
     (ensures  S.equal (hash_seq_spec_full #_ #f nhs acc actd)
@@ -540,9 +540,9 @@ let hash_seq_spec_full_even_next #_ #f j hs nhs acc actd =
 val hash_seq_spec_full_odd_next:
   #hsz:pos -> #f:MTS.tag_fun_t #hsz ->
   j:nat{j > 1} ->
-  hs:MTH.hashes #hsz {S.length hs = j} ->
-  nhs:MTH.hashes #hsz {S.length nhs = j / 2} ->
-  acc:MTH.hash #hsz -> actd:bool -> nacc:MTH.hash #hsz ->
+  hs:hashes #hsz {S.length hs = j} ->
+  nhs:hashes #hsz {S.length nhs = j / 2} ->
+  acc:hash #hsz -> actd:bool -> nacc:hash #hsz ->
   Lemma
     (requires j % 2 = 1 /\
               mt_hashes_next_rel #_ #f j hs nhs /\
@@ -571,9 +571,9 @@ let hash_seq_spec_full_odd_next #_ #f j hs nhs acc actd nacc =
 val hash_seq_spec_full_next:
   #hsz:pos -> #f:MTS.tag_fun_t #hsz ->
   j:nat{j > 1} ->
-  hs:MTH.hashes #hsz {S.length hs = j} ->
-  nhs:MTH.hashes #hsz {S.length nhs = j / 2} ->
-  acc:MTH.hash #hsz -> actd:bool -> nacc:MTH.hash #hsz -> nactd:bool ->
+  hs:hashes #hsz {S.length hs = j} ->
+  nhs:hashes #hsz {S.length nhs = j / 2} ->
+  acc:hash #hsz -> actd:bool -> nacc:hash #hsz -> nactd:bool ->
   Lemma
     (requires mt_hashes_next_rel #_ #f j hs nhs /\
               nacc == (if j % 2 = 0 then acc
@@ -592,7 +592,7 @@ val mt_rhs_inv:
   #hsz:pos -> #f:MTS.tag_fun_t #hsz ->
   j:nat ->
   smt:MTS.merkle_tree #hsz (log2c j) ->
-  rhs:MTH.hashes #hsz {S.length rhs = log2c j} ->
+  rhs:hashes #hsz {S.length rhs = log2c j} ->
   actd:bool ->
   GTot Type0 (decreases j)
 let rec mt_rhs_inv #_ #f j smt rhs actd =
@@ -607,9 +607,9 @@ let rec mt_rhs_inv #_ #f j smt rhs actd =
 
 val mt_root_inv:
   #hsz:pos -> #f:MTS.tag_fun_t #hsz ->
-  hs0:MTH.hashes #hsz {S.length hs0 > 0} ->
-  acc:MTH.hash #hsz -> actd:bool ->
-  rt:MTH.hash #hsz ->
+  hs0:hashes #hsz {S.length hs0 > 0} ->
+  acc:hash #hsz -> actd:bool ->
+  rt:hash #hsz ->
   GTot Type0
 let mt_root_inv #_ #f hs0 acc actd rt =
   MTS.mt_get_root #_ #f #(log2c (S.length hs0))
@@ -617,41 +617,41 @@ let mt_root_inv #_ #f hs0 acc actd rt =
 
 val mt_base:
   #hsz:pos -> 
-  mt:MTH.merkle_tree #hsz {MTH.mt_wf_elts mt} ->
-  olds:MTH.hashess #hsz {S.length olds = 32 /\ mt_olds_inv #_ #(MTH.MT?.tag_fun mt) 0 (MTH.MT?.i mt) olds} ->
-  GTot (bhs:MTH.hashes #hsz {S.length bhs = MTH.MT?.j mt})
+  mt:merkle_tree #hsz {mt_wf_elts mt} ->
+  olds:hashess #hsz {S.length olds = 32 /\ mt_olds_inv #_ #(MT?.tag_fun mt) 0 (MT?.i mt) olds} ->
+  GTot (bhs:hashes #hsz {S.length bhs = MT?.j mt})
 let mt_base #hsz mt olds =
-  S.head (merge_hs #hsz #(MTH.MT?.tag_fun mt) olds (MTH.MT?.hs mt))
+  S.head (merge_hs #hsz #(MT?.tag_fun mt) olds (MT?.hs mt))
 
 #pop-options // --max_fuel 1
 
 val mt_spec:
   #hsz:pos -> 
-  mt:MTH.merkle_tree #hsz {MTH.mt_wf_elts mt /\ MTH.MT?.j mt > 0} ->
-  olds:MTH.hashess{S.length olds = 32 /\ mt_olds_inv #hsz #(MTH.MT?.tag_fun mt) 0 (MTH.MT?.i mt) olds} ->
-  GTot (smt:MTS.merkle_tree #hsz (log2c (MTH.MT?.j mt)))
+  mt:merkle_tree #hsz {mt_wf_elts mt /\ MT?.j mt > 0} ->
+  olds:hashess{S.length olds = 32 /\ mt_olds_inv #hsz #(MT?.tag_fun mt) 0 (MT?.i mt) olds} ->
+  GTot (smt:MTS.merkle_tree #hsz (log2c (MT?.j mt)))
 let mt_spec #hsz mt olds =
-  hash_seq_spec #_ #(MTH.MT?.tag_fun mt) (mt_base mt olds)
+  hash_seq_spec #_ #(MT?.tag_fun mt) (mt_base mt olds)
 
 val mt_inv: 
   #hsz:pos -> 
-  mt:MTH.merkle_tree #hsz {MTH.mt_wf_elts mt} ->
-  olds:MTH.hashess{S.length olds = 32 /\ mt_olds_inv #_ #(MTH.MT?.tag_fun mt) 0 (MTH.MT?.i mt) olds} ->
+  mt:merkle_tree #hsz {mt_wf_elts mt} ->
+  olds:hashess{S.length olds = 32 /\ mt_olds_inv #_ #(MT?.tag_fun mt) 0 (MT?.i mt) olds} ->
   GTot Type0
 let mt_inv #hsz mt olds =
-  let i = MTH.MT?.i mt in
-  let j = MTH.MT?.j mt in
-  let hs = MTH.MT?.hs mt in
-  let rhs = MTH.MT?.rhs mt in
-  let f = MTH.MT?.tag_fun mt in
+  let i = MT?.i mt in
+  let j = MT?.j mt in
+  let hs = MT?.hs mt in
+  let rhs = MT?.rhs mt in
+  let f = MT?.tag_fun mt in
   let fhs = merge_hs #hsz #f olds hs in
-  let rt = MTH.MT?.mroot mt in
+  let rt = MT?.mroot mt in
   log2c_bound j 32;
   mt_olds_hs_inv #_ #f 0 i j olds hs /\
-  (if j > 0 && MTH.MT?.rhs_ok mt
+  (if j > 0 && MT?.rhs_ok mt
   then (mt_olds_hs_lth_inv_ok #_ #f 0 i j olds hs;
        mt_hashes_lth_inv_log_converted #_ #f j fhs;
        (mt_rhs_inv #_ #f j (mt_spec mt olds) (S.slice rhs 0 (log2c j)) false /\
-       mt_root_inv #_ #f (mt_base mt olds) MTH.hash_init false rt))
+       mt_root_inv #_ #f (mt_base mt olds) hash_init false rt))
   else true)
 
